\documentclass[12pt]{standalone}

\usepackage[utf8x]{inputenc}
\usepackage[T1]{fontenc}

\usepackage{amsmath, amssymb}

\begin{document}
    \begin{minipage}{9cm}

        \begin{tabular}{|c|}
        \hline
        \\

            \vbox{\begin{equation*}
            f(m, x) = sign \cdot ((1 + (b - 1) \frac{m}{2^{M}}) \cdot b^{x} - a) \cdot c
            \end{equation*}}

        \\

            \vbox{\begin{equation*}
            \{ m \in \mathbb{Z} \mid 0 \leq m < 2^{M} \}
            \end{equation*}}

        \\

            \vbox{\begin{equation*}\tag{4 bits}
            \{ x \in \mathbb{Z} \mid -8 \leq x \leq 7 \},
            \quad
            b = 2
            \end{equation*}}

        \\

            \vbox{\begin{equation*}\tag{3 bits}
            \{ x \in \mathbb{Z} \mid -6 \leq x \leq 1 \},
            \quad
            b = 2
            \end{equation*}}

        \\

            \vbox{\begin{equation*}\tag{2 bits}
            \{ x \in \mathbb{Z} \mid -3 \leq x \leq 0 \},
            \quad
            b = 3
            \end{equation*}}

        \\

            \vbox{\begin{equation*}
            a = (1 + (b - 1) \frac{0}{2^{M}}) \cdot b^{\min{X}}
            \quad \quad
            a = b^{\min{X}}
            \end{equation*}}

        \\

            \vbox{\begin{equation*}
            c = \frac{1}{1 - a}
            \end{equation*}}

        \\
        \hline
        \end{tabular}

    \end{minipage}
\end{document}
